extraction: Move redefined bits out of MicroBenchmarks

src/CertifiedExtraction/Benchmarks/MicroEncoders.v
@@ -1,8 +1,5 @@
 Require Import Benchmarks.MicroEncodersSetup.
 
-
-Require Import Fiat.BinEncoders.Env.Common.Compose.
-
 Record FourWords :=
   { w0 : BoundedNat 8;
     w1 : BoundedNat 8;
@@ -16,17 +13,6 @@ Definition ListOfNat_encode (ls : BoundedList (BoundedNat 8) 256) :=
   fst (((encode_word_Impl WO~0~0~1~0~1~0~1~0) ThenC
         (encode_nat_Impl 8 (length (projT1 ls))) ThenC
         (encode_list_Impl (fun n : BoundedNat _ => encode_nat_Impl 8 (projT1 n)) (projT1 ls))) tt).
-Section Nat.
-  Context {B : Type}.
-  Context {cache : Cache}.
-  Context {cacheAddNat : CacheAdd cache nat}.
-  Context {transformer : Transformer B}.
-  Context {transformerUnit : TransformerUnitOpt transformer bool}.
-
-  Definition EncodeBoundedNat {k} (n : BoundedNat k) (ce : CacheEncode) : B * CacheEncode :=
-    (* NToWord + N.of_nat needed for performance (otherwise apply doesn't terminate) *)
-    encode_word_Impl (@NToWord k (N.of_nat (`n))) ce.
-End Nat.
 
 Definition FourWords_encode (t : FourWords) :=
 byteString
@@ -49,293 +35,11 @@ Definition FourWordsAsCollectionOfVariables
 Hint Unfold FourWords_encode : f2f_binencoders_autorewrite_db.
 Hint Unfold FourWordsAsCollectionOfVariables : f2f_binencoders_autorewrite_db.
 
-Lemma CompileCallAllocString {real_capacity}: (* FIXME replace existing with this *)
-  forall (vcapacity vstream : string) (tenv tenv' : Telescope ADTValue)
-    ext (env : GLabelMap.t (FuncSpec ADTValue)) capacity,
-    let wrapper := WrapInstance (H := (@WrapListByte real_capacity)) in
-    forall pNext pArg fAllocString,
-      vcapacity <> vstream ->
-      vstream ∉ ext ->
-      NotInTelescope vstream tenv ->
-      IL.goodSize (2 + Word.wordToNat capacity * 4) ->
-      real_capacity = Word.wmult capacity (Word.natToWord 32 4) ->
-      GLabelMap.MapsTo fAllocString (Axiomatic BytesADTSpec.New) env ->
-      {{ [[ ` vstream ->> nil as _]]::tenv }}
-        pNext
-      {{ [[ ` vstream ->> nil as _]]::tenv' }} ∪ {{ ext }} // env ->
-      {{ tenv }}
-        pArg
-      {{ [[ ` vcapacity ->> capacity as _ ]] :: tenv }} ∪ {{ ext }} // env ->
-      {{ tenv }}
-        Seq (Seq pArg (Call vstream fAllocString [vcapacity])) pNext
-      {{ [[ ` vstream ->> nil as _]]::tenv' }} ∪ {{ ext }} // env.
-Proof.
-Admitted.
-
-Lemma encode_char' :
-  forall w, encode_word' 8 w =
-       {| front := WO;
-          paddingOK := Lt.lt_0_Sn _;
-          byteString := w :: nil |}.
-Proof.
-  intros; change 8 with (8+0); rewrite encode_char.
-  shatter_word w; simpl; rewrite ByteString_transform_id_right.
-  reflexivity.
-Qed.
-
-Definition BoundedNat8ToByte (w: BoundedNat 8) :=
-  natToWord 8 (`w).
-
-Lemma EncodeBoundedNat8_simplify : (* {cache} {cacheAddNat : CacheAdd cache nat} : *)
-  forall (w: BoundedNat 8), (* (c: @CacheEncode cache), *)
-    EncodeBoundedNat w tt =
-    ({| padding := 0; front := WO; paddingOK := Lt.lt_0_Sn 7; byteString := (BoundedNat8ToByte w :: nil) |}, addE tt 8).
-Proof.
-  unfold EncodeBoundedNat, encode_word_Impl; intros.
-  rewrite encode_char', NToWord_of_nat.
-  reflexivity.
-Qed.
-
-Lemma zext_inj {sz} {sz'} :
-  forall (w w' : word sz),
-    (zext w sz') = (zext w' sz') ->
-    w = w'.
-Proof.
-  unfold zext; intros * H.
-  apply (f_equal (@Word.split1 _ _)) in H.
-  rewrite !split1_combine in H.
-  assumption.
-Qed.
-
-Definition BtoW (b: B) : W :=
-  (zext b 24).
-
-Lemma BtoW_inj :
-  forall (v v' : byte),
-    BtoW v = BtoW v' ->
-    v = v'.
-Proof.
-  intros; eapply zext_inj; apply H.
-Qed.
-
-Lemma WrapByte_inj {av} :
-  forall (v v' : byte),
-    SCA av (BtoW v) = SCA av (BtoW v') -> v = v'.
-Proof.
-  inversion 1; eauto using BtoW_inj.
-Qed.
-
-Instance WrapByte {av} : FacadeWrapper (Value av) byte :=
-  {| wrap b := SCA _ (BtoW b);
-     wrap_inj := WrapByte_inj |}.
-
-Ltac facade_cleanup_call ::=
-     match goal with
-     | _ => progress cbv beta iota delta [add_remove_many] in *
-     | _ => progress cbv beta iota delta [sel] in *
-     | [ H: Axiomatic ?s = Axiomatic ?s' |- _ ] => inversion H; subst; clear dependent H
-     | [ H: PreCond ?f _ |- _ ] => let hd := head_constant f in unfold hd in H; cbv beta iota delta [PreCond] in H
-     | [ H: PostCond ?f _ _ |- _ ] => let hd := head_constant f in unfold hd in H; cbv beta iota delta [PostCond] in H
-     | [  |- PreCond ?f _ ] => let hd := head_constant f in unfold hd; cbv beta iota delta [PreCond]
-     | [  |- PostCond ?f _ _ ] => let hd := head_constant f in unfold hd; cbv beta iota delta [PostCond]
-     | [ H: WeakEq ?lhs _ |- _ ] => progress learn_all_WeakEq_remove H lhs
-     | [ |- context[ListFacts4.mapM] ] => progress simpl ListFacts4.mapM
-     | [ H: context[ListFacts4.mapM] |- _ ] => progress simpl ListFacts4.mapM in H
-     | [ H: List.combine ?a ?b = _, H': List.length ?a = List.length ?b |- _ ] => learn (combine_inv a b H' H)
-     | [ |-  context[List.split (cons _ _)] ] => simpl
-     | [ H: context[List.split (cons _ _)] |- _ ] => may_touch H; simpl in H
-     | [ H: List.cons _ _ = List.cons _ _ |- _ ] =>
-       (* Not using inversion: it sometimes loops *)
-       let heads_eq := fresh in
-       destruct (List_cons_inj H) as (heads_eq & ?);
-       pose proof heads_eq;    (* Make a copy for cases where inversion goes berzerk *)
-       inversion heads_eq; try subst; clear dependent H
-     | _ => GLabelMapUtils.normalize
-     | _ => solve [GLabelMapUtils.decide_mapsto_maybe_instantiate]
-     | [  |- exists _, _ ] => eexists
-     end.
-
 Open Scope list_scope.
-
-Lemma CompileCallWrite8_base capacity :
-  let wrapper := @WrapListByte capacity in
-  forall (vtmp varg vstream : string) (stream : list byte)
-    (n : byte) fWrite8 tenv ext env,
-    (List.length stream + 1 <= wordToNat capacity)%nat ->
-    GLabelMap.MapsTo fWrite8 (Axiomatic BytesADTSpec.Push) env ->
-    Lifted_MapsTo ext tenv vstream (wrap stream) ->
-    Lifted_MapsTo ext tenv varg (wrap n) ->
-    vtmp <> vstream ->
-    vtmp ∉ ext ->
-    vstream ∉ ext ->
-    Lifted_not_mapsto_adt ext tenv vtmp ->
-    (* Lifted_not_mapsto_adt ext tenv vtmp -> *)
-    (* varg <> vstream -> *)
-    (* vtmp <> vstream -> *)
-    (* vtmp <> varg -> *)
-    (* vtmp ∉ ext -> *)
-    (* vstream ∉ ext -> *)
-    {{ tenv }}
-      Call vtmp fWrite8 (vstream :: varg :: nil)
-    {{ [[ `vtmp ->> W0 as _ ]]
-        :: [[ `vstream ->> stream ++ n :: nil as _ ]] ::
-        DropName vstream (DropName vtmp tenv) }} ∪ {{ ext }} // env.
-Proof.
-  intros.
-  repeat match goal with
-         | _ => progress (SameValues_Facade_t_step || facade_cleanup_call || LiftPropertyToTelescope_t)
-         | [  |- context[IL.BtoW] ] => replace IL.BtoW with BtoW by (clear; admit)
-         | [ H: context[IL.BtoW] |- _ ] => replace IL.BtoW with BtoW in H by (clear; admit)
-         | [ H: BtoW _ = BtoW _ |- _ ] => learn (BtoW_inj _ _ H); subst
-         end.
-  facade_eauto.
-  facade_eauto.
-  repeat apply DropName_remove; facade_eauto.
-Qed.
-
-Lemma CompileCallWrite8 capacity :
-  let wrapper := @WrapListByte capacity in
-  forall (vtmp varg vstream : string) (stream : list byte)
-    (tenv tenv' tenv'': Telescope ADTValue)
-    (n : byte) ext env
-    pArg pNext fWrite8,
-    ((|stream |) + 1 <= wordToNat capacity)%nat ->
-    PreconditionSet tenv' ext [[[vtmp; vstream; varg]]] ->
-    GLabelMap.MapsTo fWrite8 (Axiomatic BytesADTSpec.Push) env ->
-    {{ [[ ` vstream ->> stream as _]]::tenv }}
-      pArg
-    {{ [[ ` vstream ->> stream as _]]::[[ ` varg ->> n as _]]::tenv' }} ∪ {{ ext }} // env ->
-    {{ [[ ` vstream ->> stream ++ n :: nil as _]]::tenv' }}
-      pNext
-    {{ [[ ` vstream ->> stream ++ n :: nil as _]]::tenv'' }} ∪ {{ ext }} // env ->
-    {{ [[ ` vstream ->> stream as _]]::tenv }}
-      Seq pArg (Seq (Call vtmp fWrite8 [vstream; varg]) pNext)
-    {{ [[ ` vstream ->> stream ++ n :: nil as _]]::tenv'' }} ∪ {{ ext }} // env.
-Proof.
-  hoare; hoare; hoare.
-
-  PreconditionSet_t;
-    apply ProgOk_Remove_Skip_R; hoare;
-      [ apply generalized CompileCallWrite8_base | ];
-      repeat repeat match goal with
-                    | _ => progress intros
-                    | _ => apply ProgOk_Chomp_Some
-                    | _ => apply CompileDeallocSCA_discretely
-                    | _ => progress (compile_do_side_conditions || Lifted_t)
-                    end; (assumption || apply CompileSkip).
-Qed.
-
-Lemma wordToNat_inj {sz} :
-  forall (w1 w2: word sz),
-    wordToNat w1 = wordToNat w2 ->
-    w1 = w2.
-Proof.
-  intros * H.
-  apply (f_equal (@natToWord sz)) in H.
-  rewrite !natToWord_wordToNat in H.
-  assumption.
-Qed.
-
-Lemma BoundedN_BoundedNat {sz} :
-  forall x, lt x (pow2 sz) -> N.lt (N.of_nat x) (Npow2 sz).
-Proof.
-  intros.
-  apply Nomega.Nlt_in.
-  rewrite Nat2N.id, Npow2_nat.
-  assumption.
-Qed.
-
-Lemma BtoW_BoundedNat8ToByte_natToWord :
-  forall w,
-    BtoW (BoundedNat8ToByte w) = natToWord 32 (` w).
-Proof.
-  intros; apply wordToN_inj.
-  unfold BoundedNat8ToByte, BtoW, zext.
-  rewrite (InternetChecksum.wordToN_extend 8 24).
-  destruct w as (? & pr); rewrite !IL.natToWordToN.
-  - reflexivity.
-  - simpl; apply BoundedN_BoundedNat in pr;
-    etransitivity; eauto; reflexivity.
-  - apply BoundedN_BoundedNat; assumption.
-Qed.
-
-Lemma WrapByte_BoundedNat8ToByte_WrapNat8_compat :
-  forall w,
-    wrap (BoundedNat8ToByte w) = wrap w.
-Proof.
-  intros.
-  unfold wrap, WrapByte.
-  rewrite BtoW_BoundedNat8ToByte_natToWord; reflexivity.
-Qed.
-
-Lemma ByteString_transform_padding_0_left :
-  forall str1 str2,
-    padding str1 = 0 ->
-    padding (transform str1 str2) = padding str2.
-Proof.
-  intros * H; rewrite transform_padding_eq, H.
-  apply NPeano.Nat.mod_small.
-  destruct str2; assumption.
-Qed.
-
-Lemma ByteString_transform_padding_0 :
-  forall str1 str2,
-    padding str1 = 0 ->
-    padding str2 = 0 ->
-    padding (transform str1 str2) = 0.
-Proof.
-  intros * H H'; rewrite transform_padding_eq, H, H'.
-  reflexivity.
-Qed.
-
-Lemma EncodeBoundedNat8_padding_0 : (* {cache} {cacheAddNat : CacheAdd cache nat} : *)
-  forall (w: BoundedNat 8), (* (c: @CacheEncode cache), *)
-    padding (fst (EncodeBoundedNat w tt)) = 0.
-Proof.
-  intros; rewrite EncodeBoundedNat8_simplify; reflexivity.
-Qed.
-
-Lemma ProgOk_Add_snd_under_fn_ret :
-  forall {A A' B av} (f: B -> Telescope av) (g: A -> A') (kfst: NameTag av _) (cpair: A * B) tenv tenv' ext env p1 p2,
-    {{ tenv }}
-      p1
-      {{ [[ NTNone  ->>  cpair as pair ]]
-          :: [[ kfst  ->> g (fst pair) as p1 ]]
-          :: TelAppend (f (snd pair)) tenv' }} ∪ {{ ext }} // env ->
-    {{ [[ NTNone  ->>  cpair as pair ]]
-        :: [[ kfst  ->> g (fst pair) as p1 ]]
-        :: TelAppend (f (snd pair)) tenv' }}
-      p2
-      {{ [[ NTNone  ->>  cpair as pair ]]
-          :: [[ kfst  ->> g (fst pair) as p1 ]]
-          :: TelAppend (Nil) tenv' }} ∪ {{ ext }} // env ->
-    {{ tenv }}
-      (Seq p1 p2)
-      {{ [[ kfst  ->> g (fst cpair) as p1 ]] :: tenv' }} ∪ {{ ext }} // env.
-Proof.
-  intros; eapply CompileSeq; try eassumption.
-  repeat setoid_rewrite Propagate_anonymous_ret.
-  repeat setoid_rewrite Propagate_anonymous_ret in H.
-  repeat setoid_rewrite Propagate_anonymous_ret in H0.
-  assumption.
-Qed.
 
 Hint Rewrite EncodeBoundedNat8_simplify :  f2f_binencoders_autorewrite_db.
 Hint Rewrite ByteString_transformer_eq_app : f2f_binencoders_autorewrite_db.
 Hint Resolve WrapByte_BoundedNat8ToByte_WrapNat8_compat : compile_do_side_conditions_db.
-
-Ltac _compile_CallWrite :=
-  match_ProgOk
-    ltac:(fun prog pre post ext env =>
-            let post' := (eval simpl in post) in
-            lazymatch post' with
-            | Cons _ (ret (_ ++ ?arg :: nil)) _ =>
-              let vtmp := gensym "tmp" in
-              let varg := gensym "arg" in
-              lazymatch arg with
-              | BoundedNat8ToByte _ => eapply (CompileCallWrite8 _ vtmp varg)
-              end
-            end).
 
 Ltac _compile_SameWrap :=
   match_ProgOk
@@ -344,11 +48,6 @@ Ltac _compile_SameWrap :=
             | [[ ?k ->> BoundedNat8ToByte ?w as _ ]] :: ?tail =>
               rewrite (TelEq_same_wrap (BoundedNat8ToByte w) w)
             end).
-
-Ltac _compile_CallAllocString ::=
-  may_alloc_head;
-  let vtmp := gensym "tmp" in
-  eapply (CompileCallAllocString vtmp).
 
 Ltac _compile_decide_padding_0 :=
   repeat first [ reflexivity |
@@ -366,75 +65,7 @@ Ltac _compile_decide_AllocString_size :=
     unify x (natToWord sz zz); reflexivity
   end.
 
-(* Lemma ByteString_length_transform_le : *)
-(*   forall str1 str2 l1 l2 l, *)
-(*     (l1 + l2 <= l)%nat -> *)
-(*     padding str1 = 0 -> *)
-(*     padding str2 = 0 -> *)
-(*     (List.length (byteString str1) <= l1)%nat -> *)
-(*     (List.length (byteString str2) <= l2)%nat -> *)
-(*     (List.length (byteString (transform str1 str2)) <= l)%nat. *)
-(* Proof. *)
-(*   intros. *)
-(*   unfold transform, ByteStringTransformer. *)
-(*   rewrite ByteString_transformer_eq_app by assumption; simpl. *)
-(*   rewrite app_length. *)
-(*   omega. *)
-(* Qed. *)
-
-(* Open Scope nat_scope. *)
-
-(* Lemma write8_side_condition_length_EncodeBoundedNat8 : *)
-(*   forall x (w: BoundedNat 8), *)
-(*     1 <= x -> *)
-(*     List.length (byteString (fst (EncodeBoundedNat w tt))) <= x. *)
-(* Proof. *)
-(*   intros; rewrite EncodeBoundedNat8_simplify. *)
-(*   assumption. *)
-(* Qed. *)
-
-(* Lemma write8_side_condition_plus_minus : *)
-(*   forall n p, *)
-(*     n <= p -> *)
-(*     n + 1 <= S p. *)
-(* Proof. *)
-(*   intros; omega. *)
-(* Qed. *)
-
-(* Ltac t := *)
-(*   match goal with *)
-(*   |  |- context[wordToNat (natToWord _ (S ?x))] => change (wordToNat (natToWord _ (S x))) with (S x) *)
-(*   |  |- List.length _ + 1 <= _ => apply write8_side_condition_plus_minus *)
-(*   | _ => progress (change (length (byteString transform_id)) with 0) *)
-(*   | _ => eapply ByteString_length_transform_le *)
-(*   | _ => eapply write8_side_condition_length_EncodeBoundedNat8 *)
-(*   |  |- padding _ = 0 => _compile_decide_padding_0 *)
-(*   |  |- 0 <= _ => apply Le.le_refl *)
-(*   |  |- S _ <= _ => apply Le.le_refl *)
-(*   | _ => progress simpl (_ + _) *)
-(*   | _ => omega *)
-(*   end. *)
-
 Open Scope nat_scope.
-
-Lemma ByteString_transform_length :
-  forall str1 str2,
-    padding str1 = 0 ->
-    padding str2 = 0 ->
-    List.length (byteString (transform str1 str2)) =
-    List.length (byteString str1) + List.length (byteString str2).
-Proof.
-  unfold transform, ByteStringTransformer; intros.
-  rewrite ByteString_transformer_eq_app by assumption; simpl.
-  rewrite app_length; reflexivity.
-Qed.
-
-Lemma EncodeBoundedNat8_length :
-  forall (w: BoundedNat 8),
-    List.length (byteString (fst (EncodeBoundedNat w tt))) = 1.
-Proof.
-  intros; rewrite EncodeBoundedNat8_simplify; reflexivity.
-Qed.
 
 Ltac _compile_decide_write8_side_condition :=
   repeat lazymatch goal with
@@ -453,29 +84,6 @@ Ltac _compile_encode_do_side_conditions :=
   | [  |- _ = _ ^* _ ] => _compile_decide_AllocString_size
   | [  |- padding _ = 0 ] => _compile_decide_padding_0
   | [  |- List.length (byteString (?x)) + 1 <= _ ] => _compile_decide_write8_side_condition
-  end.
-
-Ltac _encode_prepare_cache ::=
-  may_alloc_head; (* Only create bindings for the cache once. *)
-  match_ProgOk
-    ltac:(fun prog pre post ext env =>
-            match post with
-            | Cons (NTSome _) (ret (byteString (fst (Compose.compose _ _ _ _)))) _ =>
-              apply ProgOk_Add_snd_under_fn_ret with (f := fun _ => Nil)
-            end).
-
-Ltac _encode_cleanup ::=
-  match goal with
-  | _ => match_ProgOk
-          ltac:(fun prog pre post ext env =>
-                  match post with
-                  | [[ ret (_, _) as _]] :: _ =>
-                    apply Propagate_anonymous_ret__fast
-                  end)
-  | _ => progress simpl
-  | _ => progress autounfold with f2f_binencoders_autorewrite_db
-  | _ => progress autorewrite with f2f_binencoders_autorewrite_db
-  | [  |- context[wordToNat (natToWord _ (S ?x))] ] => change (wordToNat (natToWord _ (S x))) with (S x)
   end.
 
 Ltac compile_encoder_step ::=
