src/CertifiedExtraction/Extraction/BinEncoders/Basics.v
@@ -1,13 +1,28 @@
 Require Export Coq.NArith.NArith.
 
 Require Export Bedrock.Memory Bedrock.Word.
-Require Import
-        Fiat.BinEncoders.Env.Lib.FixList
-        Fiat.BinEncoders.Env.BinLib.FixInt
-        Fiat.BinEncoders.Env.Lib.IList
-        Fiat.BinEncoders.Env.Common.Compose
+Require Export
+        Fiat.BinEncoders.Env.Automation.SolverOpt
         Fiat.BinEncoders.Env.BinLib.Bool
-        Fiat.BinEncoders.Env.BinLib.Enum.
+        Fiat.BinEncoders.Env.BinLib.Core
+        Fiat.BinEncoders.Env.BinLib.Enum
+        Fiat.BinEncoders.Env.BinLib.FixInt
+        Fiat.BinEncoders.Env.Common.Compose
+        Fiat.BinEncoders.Env.Common.ComposeCheckSum
+        Fiat.BinEncoders.Env.Common.ComposeIf
+        Fiat.BinEncoders.Env.Common.Specs
+        Fiat.BinEncoders.Env.Common.WordFacts
+        Fiat.BinEncoders.Env.Lib.FixList
+        Fiat.BinEncoders.Env.Lib.IList
+        Fiat.BinEncoders.Env.Lib2.Bool
+        Fiat.BinEncoders.Env.Lib2.EnumOpt
+        Fiat.BinEncoders.Env.Lib2.FixListOpt
+        Fiat.BinEncoders.Env.Lib2.NatOpt
+        Fiat.BinEncoders.Env.Lib2.NoCache
+        Fiat.BinEncoders.Env.Lib2.SumTypeOpt
+        Fiat.BinEncoders.Env.Lib2.Vector
+        Fiat.BinEncoders.Env.Lib2.WordOpt
+        Fiat.BinEncoders.Env.Lib2.IPChecksum.
 
 Unset Implicit Arguments.
 
@@ -16,3 +31,20 @@ Open Scope nat_scope.
 Notation BoundedList A size := { ls: list A | List.length ls < size }.
 Notation BoundedNat size := { n: nat | (n < pow2 size)%nat }.
 Notation BoundedN size := { n: N | (n < FixInt.exp2 size)%N }.
+
+Section Nat.
+  Context {B : Type}.
+  Context {cache : Cache}.
+  Context {cacheAddNat : CacheAdd cache nat}.
+  Context {transformer : Transformer B}.
+  Context {transformerUnit : TransformerUnitOpt transformer bool}.
+
+  (* TODO move *)
+  Definition EncodeBoundedNat {k} (n : BoundedNat k) (ce : CacheEncode) : B * CacheEncode :=
+    (* NToWord + N.of_nat needed for performance (otherwise [apply] doesn't terminate) *)
+    encode_word_Impl (@NToWord k (N.of_nat (`n))) ce.
+End Nat.
+
+(* TODO move *)
+Definition BtoW (b: B) : W :=
+  (zext b 24).
