src/CertifiedExtraction/Extraction/BinEncoders/BinEncoders.v
@@ -3,6 +3,7 @@ Require Export
         Fiat.CertifiedExtraction.Extraction.BinEncoders.Wrappers
         Fiat.CertifiedExtraction.Extraction.BinEncoders.Properties
         Fiat.CertifiedExtraction.Extraction.BinEncoders.CallRules
+        Fiat.CertifiedExtraction.Extraction.BinEncoders.CallRules.ByteString
         Fiat.CertifiedExtraction.Extraction.BinEncoders.RewriteRules.
 Unset Implicit Arguments.
 
@@ -79,6 +80,7 @@ Ltac _encode_cleanup :=
   | _ => progress simpl
   | _ => progress autounfold with f2f_binencoders_autorewrite_db
   | _ => progress autorewrite with f2f_binencoders_autorewrite_db
+  | [  |- context[wordToNat (natToWord _ (S ?x))] ] => change (wordToNat (natToWord _ (S x))) with (S x)
   end.
 
 (*  Disable the propagation of rets for this file, since we use them for structure *)
