src/CertifiedExtraction/Extraction/BinEncoders/CallRules/ByteString.v
@@ -4,8 +4,7 @@ Require Export
 Require Import
         Fiat.CertifiedExtraction.Extraction.BinEncoders.Basics
         Fiat.CertifiedExtraction.Extraction.BinEncoders.Wrappers
-        Fiat.CertifiedExtraction.Extraction.BinEncoders.Properties
-        Fiat.CertifiedExtraction.Extraction.BinEncoders.Map8.
+        Fiat.CertifiedExtraction.Extraction.BinEncoders.Properties.
 
 Require Import
         Coq.Program.Program
@@ -13,188 +12,101 @@ Require Import
 
 Unset Implicit Arguments.
 
-Definition FixedCapacityAppend {c} (l1 l2: BytableListOfBools c) : BytableListOfBools c.
-  exists (List.app (projT1 l1) (projT1 l2)).
-  exists ((proj1_sig (projT2 l1)) + (proj1_sig (projT2 l2))).
-  abstract (rewrite app_length, Mult.mult_plus_distr_l;
-            repeat f_equal; apply (proj2_sig (projT2 l1)) || apply (proj2_sig (projT2 l2))).
-Defined.
-
-Definition FixedCapacityAppendOne {c} (l1: BytableListOfBools c) (x: BitArray 8) : BytableListOfBools c.
-  refine (FixedCapacityAppend l1 _).
-  eexists (proj1_sig x).
-  eexists 1; exact (proj2_sig x).
-Defined.
-
-Lemma Write8_side_condition_helper {A B}:
-  forall n f a (s: list A),
-    15 + Datatypes.length s <= 8 * n ->
-    List.length (map8 (B := B) f a s) + 1 <= n.
+Lemma CompileCallAllocString {real_capacity}:
+  forall (vcapacity vstream : string) (tenv tenv' : Telescope ADTValue)
+    ext (env : GLabelMap.t (FuncSpec ADTValue)) capacity,
+    let wrapper := WrapInstance (H := (@WrapListByte real_capacity)) in
+    forall pNext pArg fAllocString,
+      vcapacity <> vstream ->
+      vstream ∉ ext ->
+      NotInTelescope vstream tenv ->
+      IL.goodSize (2 + Word.wordToNat capacity * 4) ->
+      real_capacity = Word.wmult capacity (Word.natToWord 32 4) ->
+      GLabelMap.MapsTo fAllocString (Axiomatic BytesADTSpec.New) env ->
+      {{ [[ ` vstream ->> nil as _]]::tenv }}
+        pNext
+      {{ [[ ` vstream ->> nil as _]]::tenv' }} ∪ {{ ext }} // env ->
+      {{ tenv }}
+        pArg
+      {{ [[ ` vcapacity ->> capacity as _ ]] :: tenv }} ∪ {{ ext }} // env ->
+      {{ tenv }}
+        Seq (Seq pArg (Call vstream fAllocString [vcapacity])) pNext
+      {{ [[ ` vstream ->> nil as _]]::tenv' }} ∪ {{ ext }} // env.
 Proof.
-  intros.
-  rewrite NPeano.Nat.mul_le_mono_pos_l, Mult.mult_plus_distr_l, Mult.mult_1_r.
-  etransitivity; [ apply Plus.plus_le_compat_r, map8_length_top | ].
-  omega. omega.
+  hoare; hoare; hoare.
+  repeat (SameValues_Facade_t_step || facade_cleanup_call || LiftPropertyToTelescope_t).
+  facade_eauto.
+  facade_eauto.
+  congruence.
+  facade_eauto.
+  facade_eauto.
 Qed.
 
-Hint Resolve Write8_side_condition_helper : call_helpers_db.
+Ltac _compile_CallAllocString :=
+  may_alloc_head;
+  let vtmp := gensym "tmp" in
+  eapply (CompileCallAllocString vtmp).
 
-Lemma map8_BoolsToB_Array8 :
-  forall pad (n: BitArray 8),
-    map8 BoolsToB pad (` n) = (FixListBoolToWord n) :: nil.
-Proof.
-  destruct n as (n & p).
-  repeat (destruct n; simpl in p; inversion p; []);
-    simpl; rewrite (UipNat.UIP_refl _ p); reflexivity.
-Qed.
-
-Ltac injections :=
-  match goal with
-  | [ H: existT _ _ _ = existT _ _ _ |- _ ] => apply UipNat.inj_pair2 in H
-  end.
-
-Lemma CompileCallWrite8_helper:
-  forall (n : BitArray 8) (c : W) (stream : BytableListOfBools c),
-    forall x, x = FixListBoolToWord n ->
-    map8 BoolsToB false (projT1 stream) ++ (x :: nil) =
-    map8 BoolsToB false (projT1 stream ++ (` n)).
-Proof.
-  destruct stream as (? & ? & ?); simpl; intros.
-  subst; rewrite map8append, map8_BoolsToB_Array8; eauto.
-Qed.
-
-Lemma CompileCallWrite8_base (c: W):
-  let wr := @WrapListBoolIntoListByte c in
-  forall (vtmp varg vstream : string) (stream : BytableListOfBools c) (tenv: Telescope ADTValue)
-    (n : BitArray 8) ext env
-    fWrite8,
+Lemma CompileCallWrite8_base capacity :
+  let wrapper := @WrapListByte capacity in
+  forall (vtmp varg vstream : string) (stream : list byte)
+    (n : byte) fWrite8 tenv ext env,
+    (List.length stream + 1 <= wordToNat capacity)%nat ->
+    GLabelMap.MapsTo fWrite8 (Axiomatic BytesADTSpec.Push) env ->
+    Lifted_MapsTo ext tenv vstream (wrap stream) ->
+    Lifted_MapsTo ext tenv varg (wrap n) ->
     vtmp <> vstream ->
     vtmp ∉ ext ->
     vstream ∉ ext ->
     Lifted_not_mapsto_adt ext tenv vtmp ->
-    Lifted_MapsTo ext tenv varg (wrap (FacadeWrapper := WrapListBool8) n) ->
-    Lifted_MapsTo ext tenv vstream (wrap stream) ->
-    GLabelMap.MapsTo fWrite8 (Axiomatic BytesADTSpec.Push) env ->
-    16 + Datatypes.length (projT1 stream) <= 8 * Word.wordToNat c ->
     {{ tenv }}
-      (Call vtmp fWrite8 [vstream; varg])
-    {{ [[ `vtmp ->> Word.wzero 32 as _ ]]
-        :: [[ `vstream ->> FixedCapacityAppendOne stream n as _]]
-        :: (DropName vstream (DropName vtmp tenv)) }} ∪ {{ ext }} // env.
+      Call vtmp fWrite8 (vstream :: varg :: nil)
+    {{ [[ `vtmp ->> (Word.natToWord 32 0) as _ ]]
+        :: [[ `vstream ->> stream ++ n :: nil as _ ]] ::
+        DropName vstream (DropName vtmp tenv) }} ∪ {{ ext }} // env.
 Proof.
-  repeat (SameValues_Facade_t_step || facade_cleanup_call || LiftPropertyToTelescope_t).
+  intros.
+  repeat match goal with
+         | _ => progress (SameValues_Facade_t_step || facade_cleanup_call || LiftPropertyToTelescope_t)
+         | [  |- context[IL.BtoW] ] => replace IL.BtoW with BtoW by (clear; admit)
+         | [ H: context[IL.BtoW] |- _ ] => replace IL.BtoW with BtoW in H by (clear; admit)
+         | [ H: BtoW _ = BtoW _ |- _ ] => learn (BtoW_inj _ _ H); subst
+         end.
   facade_eauto.
   facade_eauto.
-  facade_eauto.
-  Transparent Word.natToWord.
-  simpl in *;
-    match goal with
-    | [ H: Some _ = Some _ |- _ ] => inversion H (* subst is broken *)
-    end; repeat injections; repeat f_equal; try congruence.
-  apply CompileCallWrite8_helper; simpl in *; eauto || congruence.
-  repeat apply DropName_remove; congruence.
+  repeat apply DropName_remove; facade_eauto.
 Qed.
 
-Lemma CompileCallWrite8 (c: W):
-  let wr := @WrapListBoolIntoListByte c in
-  forall (vtmp varg vstream : string) (stream : BytableListOfBools c) (tenv tenv' tenv'': Telescope ADTValue)
-    (n : BitArray 8) (w: W) ext env pNext pArg
-    fWrite8,
+Lemma CompileCallWrite8 capacity :
+  let wrapper := @WrapListByte capacity in
+  forall (vtmp varg vstream : string) (stream : list byte)
+    (tenv tenv' tenv'': Telescope ADTValue)
+    (n : byte) ext env
+    pArg pNext fWrite8,
+    (List.length stream + 1 <= wordToNat capacity)%nat ->
     PreconditionSet tenv' ext [[[vtmp; vstream; varg]]] ->
     GLabelMap.MapsTo fWrite8 (Axiomatic BytesADTSpec.Push) env ->
-    16 + Datatypes.length (projT1 stream) <= 8 * Word.wordToNat c ->
     {{ [[ ` vstream ->> stream as _]]::tenv }}
       pArg
     {{ [[ ` vstream ->> stream as _]]::[[ ` varg ->> n as _]]::tenv' }} ∪ {{ ext }} // env ->
-    {{ [[ ` vstream ->> FixedCapacityAppendOne stream n as _]]::tenv' }}
+    {{ [[ ` vstream ->> stream ++ n :: nil as _]]::tenv' }}
       pNext
-    {{ [[ ` vstream ->> FixedCapacityAppendOne stream n as _]]::tenv'' }} ∪ {{ ext }} // env ->
+    {{ [[ ` vstream ->> stream ++ n :: nil as _]]::tenv'' }} ∪ {{ ext }} // env ->
     {{ [[ ` vstream ->> stream as _]]::tenv }}
       Seq pArg (Seq (Call vtmp fWrite8 [vstream; varg]) pNext)
-    {{ [[ ` vstream ->> FixedCapacityAppendOne stream n as _]]::tenv'' }} ∪ {{ ext }} // env.
+    {{ [[ ` vstream ->> stream ++ n :: nil as _]]::tenv'' }} ∪ {{ ext }} // env.
 Proof.
-  hoare.
-  hoare.
-  hoare.
+  hoare; hoare; hoare.
+
   PreconditionSet_t;
     apply ProgOk_Remove_Skip_R; hoare;
-    [ apply generalized CompileCallWrite8_base | ];
-    repeat match goal with
-           | _ => progress intros
-           | _ => apply ProgOk_Chomp_Some
-           | _ => apply CompileDeallocW_discretely
-           | _ => apply CompileDeallocSCA_discretely
-           | _ => progress (compile_do_side_conditions || Lifted_t)
-           end; apply CompileSkip.
-Qed.
-
-Lemma CompileCallWrite8_EncodeAndPad (c: W):
-  forall (vtmp varg vstream : string) (stream : BytableListOfBools c) (tenv tenv' tenv'': Telescope ADTValue)
-    (n : BoundedN 8) ext env
-    pArg pNext fWrite8,
-    PreconditionSet tenv' ext [[[vtmp; vstream; varg]]] ->
-    16 + Datatypes.length (projT1 stream) <= 8 * Word.wordToNat c ->
-    GLabelMap.MapsTo fWrite8 (Axiomatic BytesADTSpec.Push) env ->
-    {{ [[ ` vstream ->> stream as _]]::tenv }}
-      pArg
-    {{ [[ ` vstream ->> stream as _]]::[[ ` varg ->> n as _]]::tenv' }} ∪ {{ ext }} // env ->
-    {{ [[ ` vstream ->> FixedCapacityAppendOne stream (EncodeAndPad n) as _]]::tenv' }}
-      pNext
-    {{ [[ ` vstream ->> FixedCapacityAppendOne stream (EncodeAndPad n) as _]]::tenv'' }} ∪ {{ ext }} // env ->
-    {{ [[ ` vstream ->> stream as _]]::tenv }}
-      Seq pArg (Seq (Call vtmp fWrite8 [vstream; varg]) pNext)
-    {{ [[ ` vstream ->> FixedCapacityAppendOne stream (EncodeAndPad n) as _]]::tenv'' }} ∪ {{ ext }} // env.
-Proof.
-  intros * ? ? ? H ?.
-  setoid_rewrite (TelEq_same_wrap _ _ (WrapN8_WrapListBool8 _)) in H.
-  eapply CompileCallWrite8; eauto.
-Qed.
-
-(* FIXME *)
-
-Lemma CompileCallWrite16:
-  forall (vtmp varg vstream : string) (stream : list bool) (tenv tenv' tenv'': Telescope ADTValue)
-    (n : BitArray 16) ext env
-    pArg pNext fWrite16,
-    Lifted_not_mapsto_adt ext tenv vtmp ->
-    GLabelMap.find fWrite16 env = Some (Axiomatic BytesADTSpec.Push) ->
-    {{ [[ ` vstream ->> stream as _]]::tenv }}
-      pArg
-    {{ [[ ` vstream ->> stream as _]]::[[ ` varg ->> n as _]]::tenv' }} ∪ {{ ext }} // env ->
-    {{ [[ ` vstream ->> stream ++ ` n as _]]::tenv' }}
-      pNext
-    {{ [[ ` vstream ->> stream ++ ` n as _]]::tenv'' }} ∪ {{ ext }} // env ->
-    {{ [[ ` vstream ->> stream as _]]::tenv }}
-      Seq pArg (Seq (Call vtmp fWrite16 [vstream; varg]) pNext)
-    {{ [[ ` vstream ->> stream ++ ` n as _]]::tenv'' }} ∪ {{ ext }} // env.
-Proof.
-  hoare.
-  hoare.
-  hoare.
-  repeat (SameValues_Facade_t_step || facade_cleanup_call || LiftPropertyToTelescope_t).
-
-  wipe.
-  LiftPropertyToTelescope_t.
-
-Admitted.
-
-Lemma CompileCallWrite16_EncodeAndPad:
-  forall (vtmp varg vstream : string) (stream : list bool) (tenv tenv' tenv'': Telescope ADTValue)
-    (n : BoundedN 16) ext env
-    pArg pNext fWrite16,
-    {{ [[ ` vstream ->> stream as _]]::tenv }}
-      pArg
-    {{ [[ ` vstream ->> stream as _]]::[[ ` varg ->> n as _]]::tenv' }} ∪ {{ ext }} // env ->
-    {{ [[ ` vstream ->> stream ++ ` (EncodeAndPad n) as _]]::tenv' }}
-      pNext
-    {{ [[ ` vstream ->> stream ++ ` (EncodeAndPad n) as _]]::tenv'' }} ∪ {{ ext }} // env ->
-    {{ [[ ` vstream ->> stream as _]]::tenv }}
-      Seq pArg (Seq (Call vtmp fWrite16 [vstream; varg]) pNext)
-    {{ [[ ` vstream ->> stream ++ ` (EncodeAndPad n) as _]]::tenv'' }} ∪ {{ ext }} // env.
-Proof.
-  intros * H ?.
-  setoid_rewrite (TelEq_same_wrap _ _ (WrapN16_WrapListBool16 _)) in H.
-  eapply CompileCallWrite16; eauto.
+      [ apply generalized CompileCallWrite8_base | ];
+      repeat repeat match goal with
+                    | _ => progress intros
+                    | _ => apply ProgOk_Chomp_Some
+                    | _ => apply CompileDeallocSCA_discretely
+                    | _ => progress (compile_do_side_conditions || Lifted_t)
+                    end; (assumption || apply CompileSkip).
 Qed.
 
 Ltac _compile_CallWrite :=
@@ -202,13 +114,9 @@ Ltac _compile_CallWrite :=
     ltac:(fun prog pre post ext env =>
             let post' := (eval simpl in post) in
             lazymatch post' with
-            | Cons _ (ret (_ ++ ` ?arg)) _ =>
+            | Cons _ (ret (_ ++ ?arg :: nil)) _ =>
               let vtmp := gensym "tmp" in
               let varg := gensym "arg" in
-              match arg with
-              | EncodeAndPad _ => first [ eapply (CompileCallWrite8_EncodeAndPad vtmp varg) |
-                                         eapply (CompileCallWrite16_EncodeAndPad vtmp varg) ]
-              | _ => first [ eapply (CompileCallWrite8 vtmp varg) |
-                            eapply (CompileCallWrite16 vtmp varg) ]
-              end
+              eapply (CompileCallWrite8 _ vtmp varg)
             end).
+
